Turned into Isar theories.

src/HOL/ex/Qsort.thy
@@ -6,28 +6,58 @@
 Quicksort
 *)
 
-Qsort = Sorting +
+theory Qsort = Sorting:
 
 (*Version one: higher-order*)
-consts qsort :: "((['a,'a] => bool) * 'a list) => 'a list"
+consts qsort :: "('a \<Rightarrow> 'a => bool) * 'a list \<Rightarrow> 'a list"
 
 recdef qsort "measure (size o snd)"
-    simpset "simpset() addsimps [length_filter RS le_less_trans]"
-    
-    "qsort(le, [])   = []"
-    
-    "qsort(le, x#xs) = qsort(le, [y:xs . ~ le x y])  
-                       @ (x # qsort(le, [y:xs . le x y]))"
+"qsort(le, [])   = []"
+"qsort(le, x#xs) = qsort(le, [y:xs . ~ le x y]) @ [x] @
+                   qsort(le, [y:xs . le x y])"
+(hints recdef_simp: length_filter[THEN le_less_trans])
+
+lemma qsort_permutes[simp]:
+ "multiset (qsort(le,xs)) x = multiset xs x"
+by (induct le xs rule: qsort.induct, auto)
+
+
+(*Also provable by induction*)
+lemma set_qsort[simp]: "set (qsort(le,xs)) = set xs";
+by(simp add: set_via_multiset)
+
+lemma sorted_qsort:
+ "total(le) ==> transf(le) ==> sorted le (qsort(le,xs))"
+apply (induct le xs rule: qsort.induct)
+ apply simp
+apply simp
+apply(unfold Sorting.total_def Sorting.transf_def)
+apply blast
+done
 
 
 (*Version two: type classes*)
+
 consts quickSort :: "('a::linorder) list => 'a list"
 
 recdef quickSort "measure size"
-    simpset "simpset() addsimps [length_filter RS le_less_trans]"
-    
-    "quickSort []   = []"
-    
-    "quickSort (x#l) = quickSort [y:l. ~ x<=y] @ (x # quickSort [y:l. x<=y])"
+"quickSort []   = []"
+"quickSort (x#l) = quickSort [y:l. ~ x<=y] @ [x] @ quickSort [y:l. x<=y]"
+(hints recdef_simp: length_filter[THEN le_less_trans])
+
+lemma quickSort_permutes[simp]:
+ "multiset (quickSort xs) z = multiset xs z"
+by (induct xs rule: quickSort.induct) auto
+
+(*Also provable by induction*)
+lemma set_quickSort[simp]: "set (quickSort xs) = set xs"
+by(simp add: set_via_multiset)
+
+lemma sorted_quickSort: "sorted (op <=) (quickSort xs)"
+apply (induct xs rule: quickSort.induct)
+ apply simp
+apply simp
+apply(blast intro: linorder_linear[THEN disjE] order_trans)
+done
 
 end
