src/HOL/ex/InSort.thy
@@ -6,17 +6,43 @@
 Insertion sort
 *)
 
-InSort  =  Sorting +
+theory InSort  =  Sorting:
 
 consts
-  ins :: [['a,'a]=>bool, 'a, 'a list] => 'a list
-  insort :: [['a,'a]=>bool, 'a list] => 'a list
+  ins :: "('a \<Rightarrow> 'a \<Rightarrow> bool) \<Rightarrow> 'a \<Rightarrow> 'a list \<Rightarrow> 'a list"
+  insort :: "('a \<Rightarrow> 'a \<Rightarrow> bool) \<Rightarrow> 'a list \<Rightarrow> 'a list"
 
 primrec
   "ins le x [] = [x]"
   "ins le x (y#ys) = (if le x y then (x#y#ys) else y#(ins le x ys))"
+
 primrec
   "insort le [] = []"
   "insort le (x#xs) = ins le x (insort le xs)"
+
+
+lemma multiset_ins[simp]:
+ "\<And>y. multiset(ins le x xs) y = multiset (x#xs) y"
+by (induct "xs") auto
+
+lemma insort_permutes[simp]:
+ "\<And>x. multiset(insort le xs) x = multiset xs x";
+by (induct "xs") auto
+
+lemma set_ins[simp]: "set(ins le x xs) = insert x (set xs)"
+by (simp add: set_via_multiset) fast
+
+lemma sorted_ins[simp]:
+ "\<lbrakk> total le; transf le \<rbrakk> \<Longrightarrow> sorted le (ins le x xs) = sorted le xs";
+apply (induct xs)
+apply simp_all
+apply (unfold Sorting.total_def Sorting.transf_def)
+apply blast
+done
+
+lemma sorted_insort:
+ "[| total(le); transf(le) |] ==>  sorted le (insort le xs)"
+by (induct xs) auto
+
 end
 
